coqjit/assume_insertion.v
@@ -1,0 +1,86 @@
+(* Assume insertion: inserting Assume instructions *)
+(* A pass of the middle-end optimizer *)
+(* To insert an assume, you need a guard (what to speculate on) *)
+(* And you need a label where there is an anchor, that you want to copy the metadata of *)
+(* And the Assume is inserted next to that Anchor instruction *)
+
+Require Import List.
+Require Import Coqlib.
+Require Import Maps.
+Require Import IR.
+Require Import Coq.MSets.MSetPositive.
+Require Import def_regs.
+Require Import common.
+Require Import Errors.
+Require Import monad.
+
+(** * Guard checking  *)
+(* To ensure that the Assume does not intriduce bugs, *)
+(* We check that the guard can evaluate without errors *)
+Definition check_reg (r:reg) (def:regset) : bool :=
+  PositiveSet.mem r def.
+
+Definition check_expr (e:expr) (def:regset) : bool :=
+  match e with
+  | BIN bop r1 r2 => andb (check_reg r1 def) (check_reg r2 def)
+  | UNA uop r => check_reg r def
+  | ZAR z => true
+  end.
+
+
+(* making sure that the guard can evaluate, given a set of defined registers *)
+(* Fixpoint check_guard (guard:list expr) (def:regset): bool := *)
+(*   match guard with *)
+(*   | nil => true *)
+(*   | e::guard' => *)
+(*     andb (check_expr e def) (check_guard guard' def) *)
+(*   end.    *)
+(* DEPRECATED until we allow lists of guards *)
+
+
+(** * The optimization that inserts Assume directly after an Anchor *)
+
+(* Verify that the assume can be inserted: no code between assume and anchor *)
+Definition validator (v:version) (anc_lbl: label) (guard:expr) (params: list reg): res unit :=
+  match ((ver_code v) # anc_lbl) with
+  | Some (Anchor _ _ next) =>
+    do abs <- try_op (defined_regs_analysis (ver_code v) params (ver_entry v)) "Def_regs analysis failed";
+      do def_regs <- OK(def_absstate_get anc_lbl abs);
+      match def_regs with
+      | DefFlatRegset.Inj def =>
+        match (check_expr guard def) with
+        | true => OK tt
+        | false => Error ((MSG "The guard might evaluate to an error")::nil)
+        end
+      | DefFlatRegset.Top => Error ((MSG "The analysis couldn't get the exact set of defined registers: TOP")::nil)
+      | DefFlatRegset.Bot => Error ((MSG "The analysis couldn't get the exact set of defined registers: BOT")::nil)
+      end
+  | _ => Error ((MSG "Not pointing to a valid Anchor")::nil)
+  end.
+
+(* Returns the version where the Assume has been inserted *)
+Definition insert_assume_version (v:version) (fid:fun_id) (guard:expr) (ancl:label) (params:list reg): res version :=
+  do code <- OK(ver_code v);
+    do freshlbl <- OK (fresh_sug (Pos.succ ancl) code);
+    do _ <- validator v ancl guard params; (* validating that the assume can be inserted *)
+    match (code # ancl) with
+    | Some (Anchor tgt vm next) =>
+      do instr <- try_op (code # next) "Next Label is not used in the function";
+        do update_anc <- OK (code # ancl <- (Anchor tgt vm freshlbl));
+        do new_code <- OK (update_anc # freshlbl <- (Assume guard tgt vm next));
+        (* in the new assume, the deopt target and the varmap are copied from the anchor *)
+        OK (mk_version new_code (ver_entry v))
+    | _ => Error ((MSG "Not pointing to a valid Anchor")::nil)
+    end.
+
+(* The optimization pass *)
+Definition insert_assume (fid: fun_id) (guard:expr) (anc_lbl: label) (p:program): res program :=
+  do f <- try_op (find_function_ir fid p) "Function to optimize not found";
+    do v <- OK(current_version f); (* the optimized code if it exists, the base version otherwise *)
+    do newv <- insert_assume_version v fid guard anc_lbl (fn_params f);
+    do new_program <- OK (set_version p fid newv);
+    OK (new_program).
+    
+
+Definition safe_insert_assume (p:program) (fid:fun_id) (guard:expr) (anc_lbl: label): program :=
+  safe_res (insert_assume fid guard anc_lbl) p.
